

**Lesson 1.23** Using Addition for Subtraction

Think addition for subtraction. Solve each problem.

$$8 \text{ } - 4 \text{ } = \text{  } \quad 4 \text{ } + \text{ } = 8 \text{ }$$

$$10 \text{ } - 3 \text{ } = \text{ } \quad 3 \text{ } + \text{ } = 10 \text{ }$$

$$7 \text{ } - 2 \text{ } = \text{ } \quad 2 \text{ } + \text{ } = 7 \text{ }$$

$$10 \text{ } - 4 \text{ } = \text{ } \quad 4 \text{ } + \text{ } = 10 \text{ }$$

$$5 \text{ } - 1 \text{ } = \text{ } \quad 1 \text{ } + \text{ } = 5 \text{ }$$

$$8 \text{ } - 2 \text{ } = \text{ } \quad 2 \text{ } + \text{ } = 8 \text{ }$$

$$9 \text{ } - 7 \text{ } = \text{ } \quad 7 \text{ } + \text{ } = 9 \text{ }$$

$$7 \text{ } - 6 \text{ } = \text{ } \quad 6 \text{ } + \text{ } = 7 \text{ }$$

$$8 \text{ } - 5 \text{ } = \text{ } \quad 5 \text{ } + \text{ } = 8 \text{ }$$